theories/simplang/gen_adequacy.v
@@ -55,7 +55,7 @@ End ctx_rel.
 (** Generic adequacy theorem for sheap-based logical relations. *)
 Section adequacy.
   Lemma simplang_adequacy `{sheapGpreS Σ} p_t p_s :
-    isat (∀ `(sheapGS Σ), ∃ `(sheapInv Σ) loc_rel,
+    isat (∀ `(sheapGS Σ), |==> ∃ `(sheapInv Σ) loc_rel,
       sheap_inv p_s state_empty [Call ##"main" #()] ∗
       ext_rel 0 #() #() ∗
       (∀ v_t v_s, ext_rel 0 v_t v_s -∗ gen_val_rel loc_rel v_t v_s) ∗
@@ -67,7 +67,7 @@ Section adequacy.
     intros σ_t σ_s. eapply sat_bupd, sat_mono, Hsat. clear Hsat.
     iIntros "Hprog_rel".
     iMod sheap_init as (HsheapGS) "Hinit".
-    iDestruct ("Hprog_rel" $! HsheapGS) as (HsheapInv loc_rel) "(Hinv & Hunit & Hobs & Hprog_rel)".
+    iMod ("Hprog_rel" $! HsheapGS) as (HsheapInv loc_rel) "(Hinv & Hunit & Hobs & Hprog_rel)".
     iDestruct ("Hinit" $! HsheapInv) as "[Hstate Hprogs_are]".
     iModIntro. iExists sheapGS_simulirisGS.
     iFrame "Hprog_rel Hprogs_are Hunit".
